Tidied up ORSet theory, removed clutter and reduced sizes of proofs

src/ORSet.thy
@@ -3,77 +3,42 @@ theory
 imports
   Network
 begin
-
-fun opt_default :: "'a option \<Rightarrow> 'a \<Rightarrow> 'a" (infix "default to" 50) where
+  
+fun opt_default :: "'a option \<Rightarrow> 'a \<Rightarrow> 'a" where
   "opt_default (Some x) _ = x" |
   "opt_default  None    x = x"
 
-datatype 'elem operation
-  = Add 'elem
-  | Rem 'elem
+datatype 'a operation = Add 'a | Rem 'a
 
-type_synonym 'elem state = "'elem \<rightharpoonup> 'elem operation set"
+type_synonym 'a state = "'a \<rightharpoonup> 'a operation set"
 
 locale orset_base = network_with_ops msg_id history interp "Map.empty"
-  for msg_id :: "'elem operation \<Rightarrow> 'a"
-  and history :: "nat \<Rightarrow> 'elem operation event list"
-  and interp :: "'elem operation \<Rightarrow> 'elem state \<rightharpoonup> 'elem state"
+  for msg_id :: "'a operation \<Rightarrow> 'a" and history :: "nat \<Rightarrow> 'a operation event list"
+    and interp :: "'a operation \<Rightarrow> 'a state \<rightharpoonup> 'a state"
 
 definition op_elem where
   "op_elem oper \<equiv> case oper of Add e \<Rightarrow> e | Rem e \<Rightarrow> e"
 
-definition (in orset_base) interpret_op :: "'elem operation \<Rightarrow> 'elem state \<rightharpoonup> 'elem state" ("\<langle>_\<rangle>" [0] 1000) where
-  "interpret_op oper state = (
-    let before = (state (op_elem oper)) default to {} in
-    let after = case oper of
-      Add e \<Rightarrow> before \<union> {oper} |
-      Rem e \<Rightarrow> {add \<in> before. \<not> hb add oper}
-    in Some (state ((op_elem oper) \<mapsto> after)))"
+definition (in orset_base) interpret_op :: "'a operation \<Rightarrow> 'a state \<rightharpoonup> 'a state" ("\<langle>_\<rangle>" [0] 1000) where
+  "interpret_op oper state \<equiv>
+     let before = opt_default (state (op_elem oper)) {};
+         after  = case oper of Add e \<Rightarrow> before \<union> {oper} | Rem e \<Rightarrow> {add \<in> before. \<not> hb add oper}
+     in  Some (state ((op_elem oper) \<mapsto> after))"
 
 locale orset = orset_base _ _ "orset_base.interpret_op history"
 
-lemma map_assign_commute:
-  assumes "k1 \<noteq> k2"
-  shows "(\<lambda>x. Some (x(k1 \<mapsto> f (x k1 default to {}), k2 \<mapsto> g (x k2 default to {})))) =
-         (\<lambda>x. Some (x(k2 \<mapsto> g (x k2 default to {}), k1 \<mapsto> f (x k1 default to {}))))"
-  using assms apply -
-  apply(subgoal_tac "\<And>x y. x = y \<Longrightarrow>
-         x(k1 \<mapsto> f (x k1 default to {}), k2 \<mapsto> g (x k2 default to {})) =
-         y(k2 \<mapsto> g (y k2 default to {}), k1 \<mapsto> f (y k1 default to {}))")
-  apply auto
-done
-
 lemma (in orset) add_add_commute:
   shows "\<langle>Add e1\<rangle> \<rhd> \<langle>Add e2\<rangle> = \<langle>Add e2\<rangle> \<rhd> \<langle>Add e1\<rangle>"
-  apply(unfold interpret_op_def op_elem_def kleisli_def)
-  apply(clarsimp)
-  apply(case_tac "e1=e2", simp)
-  apply(auto split: if_split_asm)
-  using map_assign_commute apply fastforce
-done
+  by(auto simp add: interpret_op_def op_elem_def kleisli_def, fastforce)
 
 lemma (in orset) add_rem_commute:
   assumes "\<not> hb (Add e1) (Rem e2) \<and> \<not> hb (Rem e2) (Add e1)"
   shows "\<langle>Add e1\<rangle> \<rhd> \<langle>Rem e2\<rangle> = \<langle>Rem e2\<rangle> \<rhd> \<langle>Add e1\<rangle>"
-  using assms apply(unfold interpret_op_def op_elem_def kleisli_def)
-  apply(clarsimp)
-  apply(case_tac "e1=e2", simp)
-  apply(subgoal_tac "\<And>x y. x = y \<Longrightarrow>
-    x(e2 \<mapsto> {add. (add = Add e2 \<or> add \<in> (x e2 default to {})) \<and> \<not> hb add (Rem e2)}) =
-    y(e2 \<mapsto> insert (Add e2) {add \<in> y e2 default to {}. \<not> hb add (Rem e2)})")
-  apply(simp)
-  using Collect_cong apply auto[1]
-  apply(simp)
-  using map_assign_commute apply fastforce
-  done
+  using assms by(cases "e1 = e2"; fastforce simp add: interpret_op_def op_elem_def kleisli_def)
 
 lemma (in orset) rem_rem_commute:
   shows "\<langle>Rem e1\<rangle> \<rhd> \<langle>Rem e2\<rangle> = \<langle>Rem e2\<rangle> \<rhd> \<langle>Rem e1\<rangle>"
-  apply(unfold interpret_op_def op_elem_def kleisli_def)
-  apply(clarsimp)
-  apply(case_tac "e1=e2", simp, simp)
-  using map_assign_commute apply fastforce
-  done
+  by(unfold interpret_op_def op_elem_def kleisli_def, fastforce)
 
 lemma (in orset) concurrent_operations_commute:
   assumes "xs prefix of i"
@@ -81,16 +46,12 @@ lemma (in orset) concurrent_operations_commute:
   using assms
   apply(clarsimp simp: hb.concurrent_ops_commute_def)
   apply(case_tac "x"; case_tac "y")
-  apply(simp add: hb.concurrent_def add_add_commute)
-  apply(simp add: hb.concurrent_def add_rem_commute)
-  apply(simp add: hb.concurrent_def add_rem_commute)
-  apply(simp add: hb.concurrent_def rem_rem_commute)
+  apply(auto simp add: hb.concurrent_def add_add_commute add_rem_commute rem_rem_commute)
 done
 
 theorem (in orset) convergence:
   assumes "set (node_deliver_messages xs) = set (node_deliver_messages ys)"
-      and "xs prefix of i"
-      and "ys prefix of j"
+      and "xs prefix of i" and "ys prefix of j"
     shows "apply_operations xs = apply_operations ys"
 using assms by(auto simp add: apply_operations_def intro: hb.convergence_ext concurrent_operations_commute
                 node_deliver_messages_distinct hb_consistent_prefix)
